finished typedefs for all EVM instruction types (including those we aren't using right now). now i just have to stitch them all together

LowLevelEvm.thy
@@ -59,7 +59,8 @@ free_constructors cases_arith_inst for
 lift_definition ARITH_INST :: "arith_inst \<Rightarrow> inst" is id by auto
 
 (* comparisons *)
-definition compare_codes :: "nat set" where "compare_codes = {n :: nat . (0x10 \<le> n \<and> n \<le> 0x15)}"
+definition compare_codes :: "nat set" where 
+  "compare_codes = set (List.upt 0x10 0x16)"
 declare compare_codes_def [simp add]
 typedef compare_inst = "compare_codes" by auto
 setup_lifting type_definition_compare_inst
@@ -73,29 +74,600 @@ lift_definition COMPARE_ISZERO :: "compare_inst" is "0x15" by auto
 
 lift_definition COMPARE_INST :: "compare_inst \<Rightarrow> inst" is id by auto
 
-definition bits_codes :: "nat set" where "bits_codes = {n :: nat . (0x16 \<le> n \<and> n \<le> 0x1f)}"
+free_constructors cases_compare_inst for
+  COMPARE_LT
+| COMPARE_GT
+| COMPARE_SLT
+| COMPARE_SGT
+| COMPARE_EQ
+| COMPARE_ISZERO
+  by(transfer;
+     auto simp del:set_upt simp add:List.upt_def)+
+
+(* bits *)
+definition bits_codes :: "nat set" where "bits_codes = set (List.upt 0x16 0x1e)"
 declare bits_codes_def [simp add]
-typedef inst_bits = "bits_codes" by auto
-setup_lifting type_definition_inst_bits
+typedef bits_inst = "bits_codes" by auto
+setup_lifting type_definition_bits_inst
 
-lift_definition BITS_AND  :: "inst_bits" is "0x16" by auto
-lift_definition BITS_OR   ::
-lift_definition BITS_XOR  ::
-lift_definition BITS_NOT  ::
-lift_definition BITS_BYTE ::
-lift_definition BITS_SHL  ::
-lift_definition BITS_SHR  ::
-lift_definition BITS_SAR  ::
+lift_definition BITS_AND  :: "bits_inst" is "0x16" by auto
+lift_definition BITS_OR   :: "bits_inst" is "0x17" by auto
+lift_definition BITS_XOR  :: "bits_inst" is "0x18" by auto
+lift_definition BITS_NOT  :: "bits_inst" is "0x19" by auto
+lift_definition BITS_BYTE :: "bits_inst" is "0x1a" by auto
+lift_definition BITS_SHL  :: "bits_inst" is "0x1b" by auto
+lift_definition BITS_SHR  :: "bits_inst" is "0x1c" by auto
+lift_definition BITS_SAR  :: "bits_inst" is "0x1d" by auto
+
+free_constructors cases_bits_inst for
+  BITS_AND
+| BITS_OR
+| BITS_XOR
+| BITS_NOT
+| BITS_BYTE
+| BITS_SHL
+| BITS_SHR
+| BITS_SAR
+  by(transfer;
+     auto simp del:set_upt simp add:List.upt_def)+
+
+(* keccak256 *)
+definition keccak256_codes  :: "nat set"  where "keccak256_codes = {0x20 :: nat}" 
+declare keccak256_codes_def [simp add]
+typedef keccak256_inst = "keccak256_codes" by auto
+setup_lifting type_definition_keccak256_inst
+
+lift_definition KECCAK256_KECCAK256 :: keccak256_inst is "0x20 :: nat" by auto
+free_constructors cases_keccak256_inst for KECCAK256_KECCAK256
+  by (transfer; auto)+
+
+(* transaction-specific data instructions *)
+definition tx_data_codes :: "nat set"
+  where 
+  "tx_data_codes = set (List.upt 0x30 0x40)"
+declare tx_data_codes_def[simp add]
+typedef tx_data_inst = tx_data_codes by auto
+setup_lifting type_definition_tx_data_inst
+
+lift_definition TX_DATA_ADDRESS        :: "tx_data_inst" is "0x30" by auto
+lift_definition TX_DATA_BALANCE        :: "tx_data_inst" is "0x31" by auto
+lift_definition TX_DATA_ORIGIN         :: "tx_data_inst" is "0x32" by auto
+lift_definition TX_DATA_CALLER         :: "tx_data_inst" is "0x33" by auto
+lift_definition TX_DATA_CALLVALUE      :: "tx_data_inst" is "0x34" by auto
+lift_definition TX_DATA_CALLDATALOAD   :: "tx_data_inst" is "0x35" by auto
+lift_definition TX_DATA_CALLDATASIZE   :: "tx_data_inst" is "0x36" by auto
+lift_definition TX_DATA_CALLDATACOPY   :: "tx_data_inst" is "0x37" by auto
+lift_definition TX_DATA_CODESIZE       :: "tx_data_inst" is "0x38" by auto
+lift_definition TX_DATA_CODECOPY       :: "tx_data_inst" is "0x39" by auto
+lift_definition TX_DATA_GASPRICE       :: "tx_data_inst" is "0x3a" by auto
+lift_definition TX_DATA_EXTCODESIZE    :: "tx_data_inst" is "0x3b" by auto
+lift_definition TX_DATA_EXTCODECOPY    :: "tx_data_inst" is "0x3c" by auto
+lift_definition TX_DATA_RETURNDATASIZE :: "tx_data_inst" is "0x3d" by auto
+lift_definition TX_DATA_RETURNDATACOPY :: "tx_data_inst" is "0x3e" by auto
+lift_definition TX_DATA_EXTCODEHASH    :: "tx_data_inst" is "0x3f" by auto
+
+free_constructors cases_tx_data_inst for
+TX_DATA_ADDRESS
+| TX_DATA_BALANCE
+| TX_DATA_ORIGIN
+| TX_DATA_CALLER
+| TX_DATA_CALLVALUE
+| TX_DATA_CALLDATALOAD
+| TX_DATA_CALLDATASIZE
+| TX_DATA_CALLDATACOPY
+| TX_DATA_CODESIZE
+| TX_DATA_CODECOPY
+| TX_DATA_GASPRICE
+| TX_DATA_EXTCODESIZE
+| TX_DATA_EXTCODECOPY
+| TX_DATA_RETURNDATASIZE
+| TX_DATA_RETURNDATACOPY
+| TX_DATA_EXTCODEHASH
+  by(transfer;
+     auto simp del:set_upt simp add:List.upt_def)+
+
+(* chain-specific data instructions *)
+definition chain_data_codes :: "nat set"
+  where
+  "chain_data_codes = set (List.upt 0x40 0x47)"
+declare chain_data_codes_def[simp add]
+typedef chain_data_inst = chain_data_codes by auto
+setup_lifting type_definition_chain_data_inst
+
+lift_definition CHAIN_DATA_BLOCKHASH   :: "chain_data_inst" is "0x40" by auto
+lift_definition CHAIN_DATA_COINBASE    :: "chain_data_inst" is "0x41" by auto
+lift_definition CHAIN_DATA_TIMESTAMP   :: "chain_data_inst" is "0x42" by auto
+lift_definition CHAIN_DATA_NUMBER      :: "chain_data_inst" is "0x43" by auto
+lift_definition CHAIN_DATA_DIFFICULTY  :: "chain_data_inst" is "0x44" by auto
+lift_definition CHAIN_DATA_CHAINID     :: "chain_data_inst" is "0x45" by auto
+lift_definition CHAIN_DATA_SELFBALANCE :: "chain_data_inst" is "0x46" by auto
+
+free_constructors cases_chain_data_inst for
+CHAIN_DATA_BLOCKHASH
+| CHAIN_DATA_COINBASE
+| CHAIN_DATA_TIMESTAMP
+| CHAIN_DATA_NUMBER
+| CHAIN_DATA_DIFFICULTY
+| CHAIN_DATA_CHAINID
+| CHAIN_DATA_SELFBALANCE
+  by(transfer;
+     auto simp del:set_upt simp add:List.upt_def)+
+
+(* state and control instructions *)
+(* we could break this down; e.g. into
+- put
+- memory ops
+- storage ops
+- resource queries
+- control flow *)
+definition state_control_codes :: "nat set" where
+"state_control_codes = set (List.upt 0x50 0x5c)"
+declare state_control_codes_def[simp add]
+typedef state_control_inst = state_control_codes by auto
+setup_lifting type_definition_state_control_inst
+
+lift_definition STATE_CONTROL_POP      :: "state_control_inst" is "0x50" by auto
+lift_definition STATE_CONTROL_MLOAD    :: "state_control_inst" is "0x51" by auto
+lift_definition STATE_CONTROL_MSTORE   :: "state_control_inst" is "0x52" by auto
+lift_definition STATE_CONTROL_MSTORE8  :: "state_control_inst" is "0x53" by auto
+lift_definition STATE_CONTROL_SLOAD    :: "state_control_inst" is "0x54" by auto
+lift_definition STATE_CONTROL_SSTORE   :: "state_control_inst" is "0x55" by auto
+lift_definition STATE_CONTROL_JUMP     :: "state_control_inst" is "0x56" by auto
+lift_definition STATE_CONTROL_JUMPI    :: "state_control_inst" is "0x57" by auto
+lift_definition STATE_CONTROL_PC       :: "state_control_inst" is "0x58" by auto
+lift_definition STATE_CONTROL_MSIZE    :: "state_control_inst" is "0x59" by auto
+lift_definition STATE_CONTROL_GAS      :: "state_control_inst" is "0x5a" by auto
+lift_definition STATE_CONTROL_JUMPDEST :: "state_control_inst" is "0x5b" by auto
+
+free_constructors cases_state_control_inst for
+STATE_CONTROL_POP
+| STATE_CONTROL_MLOAD
+| STATE_CONTROL_MSTORE
+| STATE_CONTROL_MSTORE8
+| STATE_CONTROL_SLOAD
+| STATE_CONTROL_SSTORE
+| STATE_CONTROL_JUMP
+| STATE_CONTROL_JUMPI
+| STATE_CONTROL_PC
+| STATE_CONTROL_MSIZE
+| STATE_CONTROL_GAS
+| STATE_CONTROL_JUMPDEST
+  by(transfer;
+     auto simp del:set_upt simp add:List.upt_def)+
+
+(* push instructions *)
+definition push_codes :: "nat set" where
+"push_codes = set (List.upt 0x60 0x80)"
+declare push_codes_def[simp add]
+typedef push_inst = push_codes by auto
+setup_lifting type_definition_push_inst
+
+(* we split push into two sub-groups to avoid having a 32-way free_constructors theorem *)
+definition push_few_codes :: "nat set" where
+"push_few_codes = set (List.upt 0x60 0x70)"
+declare push_few_codes_def[simp add]
+typedef push_few_inst = push_few_codes by auto
+setup_lifting type_definition_push_few_inst
+
+lift_definition PUSHF_PUSH1  :: "push_few_inst" is "0x60" by auto
+lift_definition PUSHF_PUSH2  :: "push_few_inst" is "0x61" by auto
+lift_definition PUSHF_PUSH3  :: "push_few_inst" is "0x62" by auto
+lift_definition PUSHF_PUSH4  :: "push_few_inst" is "0x63" by auto
+lift_definition PUSHF_PUSH5  :: "push_few_inst" is "0x64" by auto
+lift_definition PUSHF_PUSH6  :: "push_few_inst" is "0x65" by auto
+lift_definition PUSHF_PUSH7  :: "push_few_inst" is "0x66" by auto
+lift_definition PUSHF_PUSH8  :: "push_few_inst" is "0x67" by auto
+lift_definition PUSHF_PUSH9  :: "push_few_inst" is "0x68" by auto
+lift_definition PUSHF_PUSH10 :: "push_few_inst" is "0x69" by auto
+lift_definition PUSHF_PUSH11 :: "push_few_inst" is "0x6a" by auto
+lift_definition PUSHF_PUSH12 :: "push_few_inst" is "0x6b" by auto
+lift_definition PUSHF_PUSH13 :: "push_few_inst" is "0x6c" by auto
+lift_definition PUSHF_PUSH14 :: "push_few_inst" is "0x6d" by auto
+lift_definition PUSHF_PUSH15 :: "push_few_inst" is "0x6e" by auto
+lift_definition PUSHF_PUSH16 :: "push_few_inst" is "0x6f" by auto
+
+free_constructors cases_push_few_inst for
+PUSHF_PUSH1
+| PUSHF_PUSH2
+| PUSHF_PUSH3
+| PUSHF_PUSH4
+| PUSHF_PUSH5
+| PUSHF_PUSH6
+| PUSHF_PUSH7
+| PUSHF_PUSH8
+| PUSHF_PUSH9
+| PUSHF_PUSH10
+| PUSHF_PUSH11
+| PUSHF_PUSH12
+| PUSHF_PUSH13
+| PUSHF_PUSH14
+| PUSHF_PUSH15
+| PUSHF_PUSH16
+  by(transfer;
+     auto simp del:set_upt simp add:List.upt_def)+
+
+definition push_many_codes :: "nat set" where
+"push_many_codes = set (List.upt 0x70 0x80)"
+declare push_many_codes_def[simp add]
+typedef push_many_inst = push_many_codes by auto
+setup_lifting type_definition_push_many_inst
+
+lift_definition PUSHM_PUSH17 :: "push_many_inst" is "0x70" by auto
+lift_definition PUSHM_PUSH18 :: "push_many_inst" is "0x71" by auto
+lift_definition PUSHM_PUSH19 :: "push_many_inst" is "0x72" by auto
+lift_definition PUSHM_PUSH20 :: "push_many_inst" is "0x73" by auto
+lift_definition PUSHM_PUSH21 :: "push_many_inst" is "0x74" by auto
+lift_definition PUSHM_PUSH22 :: "push_many_inst" is "0x75" by auto
+lift_definition PUSHM_PUSH23 :: "push_many_inst" is "0x76" by auto
+lift_definition PUSHM_PUSH24 :: "push_many_inst" is "0x77" by auto
+lift_definition PUSHM_PUSH25 :: "push_many_inst" is "0x78" by auto
+lift_definition PUSHM_PUSH26 :: "push_many_inst" is "0x79" by auto
+lift_definition PUSHM_PUSH27 :: "push_many_inst" is "0x7a" by auto
+lift_definition PUSHM_PUSH28 :: "push_many_inst" is "0x7b" by auto
+lift_definition PUSHM_PUSH29 :: "push_many_inst" is "0x7c" by auto
+lift_definition PUSHM_PUSH30 :: "push_many_inst" is "0x7d" by auto
+lift_definition PUSHM_PUSH31 :: "push_many_inst" is "0x7e" by auto
+lift_definition PUSHM_PUSH32 :: "push_many_inst" is "0x7f" by auto
+
+free_constructors cases_push_few_inst for
+PUSHM_PUSH17
+| PUSHM_PUSH18
+| PUSHM_PUSH19
+| PUSHM_PUSH20
+| PUSHM_PUSH21
+| PUSHM_PUSH22
+| PUSHM_PUSH23
+| PUSHM_PUSH24
+| PUSHM_PUSH25
+| PUSHM_PUSH26
+| PUSHM_PUSH27
+| PUSHM_PUSH28
+| PUSHM_PUSH29
+| PUSHM_PUSH30
+| PUSHM_PUSH31
+| PUSHM_PUSH32
+  by(transfer;
+     auto simp del:set_upt simp add:List.upt_def)+
+
+(* putting together the pieces *)
+lift_definition PUSHF :: "push_few_inst \<Rightarrow> push_inst" is id by auto
+lift_definition PUSHM :: "push_many_inst \<Rightarrow> push_inst" is id by auto
+
+free_constructors cases_push_inst for
+PUSHF
+| PUSHM
+  by(transfer;
+     auto simp del:set_upt simp add:List.upt_def)+
+
+(* general version for use when not case-splitting.
+   we could have one of these each for PUSHM and PUSHF, but because that is an
+   artificial distinction anyway there doesn't seem to be much point *)
+fun push_gen :: "nat \<Rightarrow> nat" where
+"push_gen n =
+  0x60 + (n mod 32)"
+
+lift_definition PUSH_GEN :: "nat \<Rightarrow> push_inst" is push_gen
+proof-
+  fix n :: nat
+
+  have "n mod 32 < 32" using pos_mod_bound[of 32 n] by auto
+
+  hence Upt32: "n mod 32 \<in> set (List.upt 0 32)" by auto
+
+  hence "(0x60 + (n mod 32)) \<in> ((\<lambda> x . x + 0x60) ` set (List.upt 0 32))"
+    using Set.imageI[OF Upt32, of "(\<lambda> x . x + 0x60)"] by auto
+
+  hence Mapped : "(0x60 + (n mod 32)) \<in> set (map (\<lambda> x . x + 0x60) (List.upt 0 32))"
+    by auto
+
+  then show "push_gen n \<in> push_codes"
+    using List.map_add_upt by auto
+qed
+
+(*
+free_constructors cases_push_inst for
+PUSH_PUSH1
+| PUSH_PUSH2
+| PUSH_PUSH3
+| PUSH_PUSH4
+| PUSH_PUSH5
+| PUSH_PUSH6
+| PUSH_PUSH7
+| PUSH_PUSH8
+| PUSH_PUSH9
+| PUSH_PUSH10
+| PUSH_PUSH11
+| PUSH_PUSH12
+| PUSH_PUSH13
+| PUSH_PUSH14
+| PUSH_PUSH15
+| PUSH_PUSH16
+| PUSH_PUSH17
+| PUSH_PUSH18
+| PUSH_PUSH19
+| PUSH_PUSH20
+| PUSH_PUSH21
+| PUSH_PUSH22
+| PUSH_PUSH23
+| PUSH_PUSH24
+| PUSH_PUSH25
+| PUSH_PUSH26
+| PUSH_PUSH27
+| PUSH_PUSH28
+| PUSH_PUSH29
+| PUSH_PUSH30
+| PUSH_PUSH31
+| PUSH_PUSH32
+(* TODO: perhaps this is slower than we'd like. *)
+  by(transfer;
+     auto simp del:set_upt simp add:List.upt_def)+
+*)
+
+(* dup instructions *)
+definition dup_inst_codes :: "nat set" where
+"dup_inst_codes = set (List.upt 0x80 0x90)"
+declare dup_inst_codes_def[simp add]
+typedef dup_inst = dup_inst_codes by auto
+setup_lifting type_definition_dup_inst
+
+lift_definition DUP_DUP1  :: "dup_inst" is "0x80" by auto
+lift_definition DUP_DUP2  :: "dup_inst" is "0x81" by auto
+lift_definition DUP_DUP3  :: "dup_inst" is "0x82" by auto 
+lift_definition DUP_DUP4  :: "dup_inst" is "0x83" by auto
+lift_definition DUP_DUP5  :: "dup_inst" is "0x84" by auto
+lift_definition DUP_DUP6  :: "dup_inst" is "0x85" by auto
+lift_definition DUP_DUP7  :: "dup_inst" is "0x86" by auto
+lift_definition DUP_DUP8  :: "dup_inst" is "0x87" by auto
+lift_definition DUP_DUP9  :: "dup_inst" is "0x88" by auto
+lift_definition DUP_DUP10 :: "dup_inst" is "0x89" by auto
+lift_definition DUP_DUP11 :: "dup_inst" is "0x8a" by auto
+lift_definition DUP_DUP12 :: "dup_inst" is "0x8b" by auto
+lift_definition DUP_DUP13 :: "dup_inst" is "0x8c" by auto
+lift_definition DUP_DUP14 :: "dup_inst" is "0x8d" by auto
+lift_definition DUP_DUP15 :: "dup_inst" is "0x8e" by auto
+lift_definition DUP_DUP16 :: "dup_inst" is "0x8f" by auto
+
+(* general version for use when not case-splitting *)
+fun dup_gen :: "nat \<Rightarrow> nat" where
+"dup_gen n =
+  0x80 + (n mod 16)"
+
+lift_definition DUP_GEN :: "nat \<Rightarrow> dup_inst" is dup_gen
+proof-
+  fix n :: nat
+
+  have "n mod 16 < 16" using pos_mod_bound[of 16 n] by auto
+
+  hence Upt32: "n mod 16 \<in> set (List.upt 0 16)" by auto
+
+  hence "(0x80 + (n mod 16)) \<in> ((\<lambda> x . x + 0x80) ` set (List.upt 0 16))"
+    using Set.imageI[OF Upt32, of "(\<lambda> x . x + 0x80)"] by auto
+
+  hence Mapped : "(0x80 + (n mod 16)) \<in> set (map (\<lambda> x . x + 0x80) (List.upt 0 16))"
+    by auto
+
+  then show "dup_gen n \<in> dup_inst_codes"
+    using List.map_add_upt by auto
+qed
 
 
+free_constructors cases_dup_inst for
+DUP_DUP1
+| DUP_DUP2
+| DUP_DUP3
+| DUP_DUP4
+| DUP_DUP5
+| DUP_DUP6
+| DUP_DUP7
+| DUP_DUP8
+| DUP_DUP9
+| DUP_DUP10
+| DUP_DUP11
+| DUP_DUP12
+| DUP_DUP13
+| DUP_DUP14
+| DUP_DUP15
+| DUP_DUP16
+  by(transfer;
+     auto simp del:set_upt simp add:List.upt_def)+
 
-definition is_ADD :: "inst_arith \<Rightarrow> bool" where
-"is_ADD x \<equiv> case x of ARITH_ADD \<Rightarrow> True | _ \<Rightarrow> False"
+
+(* swap instructions *)
+definition swap_inst_codes :: "nat set" where
+"swap_inst_codes = set (List.upt 0x90 0xa0)"
+declare swap_inst_codes_def[simp add]
+typedef swap_inst = swap_inst_codes by auto
+setup_lifting type_definition_swap_inst
+
+lift_definition SWAP_SWAP1  :: "swap_inst" is "0x90" by auto
+lift_definition SWAP_SWAP2  :: "swap_inst" is "0x91" by auto
+lift_definition SWAP_SWAP3  :: "swap_inst" is "0x92" by auto 
+lift_definition SWAP_SWAP4  :: "swap_inst" is "0x93" by auto
+lift_definition SWAP_SWAP5  :: "swap_inst" is "0x94" by auto
+lift_definition SWAP_SWAP6  :: "swap_inst" is "0x95" by auto
+lift_definition SWAP_SWAP7  :: "swap_inst" is "0x96" by auto
+lift_definition SWAP_SWAP8  :: "swap_inst" is "0x97" by auto
+lift_definition SWAP_SWAP9  :: "swap_inst" is "0x98" by auto
+lift_definition SWAP_SWAP10 :: "swap_inst" is "0x99" by auto
+lift_definition SWAP_SWAP11 :: "swap_inst" is "0x9a" by auto
+lift_definition SWAP_SWAP12 :: "swap_inst" is "0x9b" by auto
+lift_definition SWAP_SWAP13 :: "swap_inst" is "0x9c" by auto
+lift_definition SWAP_SWAP14 :: "swap_inst" is "0x9d" by auto
+lift_definition SWAP_SWAP15 :: "swap_inst" is "0x9e" by auto
+lift_definition SWAP_SWAP16 :: "swap_inst" is "0x9f" by auto
+
+(* general version for use when not case-splitting *)
+fun swap_gen :: "nat \<Rightarrow> nat" where
+"swap_gen n =
+  0x90 + (n mod 16)"
+
+lift_definition SWAP_GEN :: "nat \<Rightarrow> swap_inst" is swap_gen
+proof-
+  fix n :: nat
+
+  have "n mod 16 < 16" using pos_mod_bound[of 16 n] by auto
+
+  hence Upt32: "n mod 16 \<in> set (List.upt 0 16)" by auto
+
+  hence "(0x90 + (n mod 16)) \<in> ((\<lambda> x . x + 0x90) ` set (List.upt 0 16))"
+    using Set.imageI[OF Upt32, of "(\<lambda> x . x + 0x90)"] by auto
+
+  hence Mapped : "(0x90 + (n mod 16)) \<in> set (map (\<lambda> x . x + 0x90) (List.upt 0 16))"
+    by auto
+
+  then show "swap_gen n \<in> swap_inst_codes"
+    using List.map_add_upt by auto
+qed
+
+free_constructors cases_swap_inst for
+SWAP_SWAP1
+| SWAP_SWAP2
+| SWAP_SWAP3
+| SWAP_SWAP4
+| SWAP_SWAP5
+| SWAP_SWAP6
+| SWAP_SWAP7
+| SWAP_SWAP8
+| SWAP_SWAP9
+| SWAP_SWAP10
+| SWAP_SWAP11
+| SWAP_SWAP12
+| SWAP_SWAP13
+| SWAP_SWAP14
+| SWAP_SWAP15
+| SWAP_SWAP16
+  by(transfer;
+     auto simp del:set_upt simp add:List.upt_def)+
+
+(* log instructions *)
+definition log_codes where
+"log_codes = set (List.upt 0xa0 0xa5)"
+declare log_codes_def[simp]
+typedef log_inst = log_codes by auto
+setup_lifting type_definition_log_inst
+
+lift_definition LOG_LOG0 :: "log_inst" is "0xa0" by auto
+lift_definition LOG_LOG1 :: "log_inst" is "0xa1" by auto
+lift_definition LOG_LOG2 :: "log_inst" is "0xa2" by auto
+lift_definition LOG_LOG3 :: "log_inst" is "0xa3" by auto
+lift_definition LOG_LOG4 :: "log_inst" is "0xa4" by auto
+
+free_constructors cases_log_inst for
+LOG_LOG0
+| LOG_LOG1
+| LOG_LOG2
+| LOG_LOG3
+| LOG_LOG4
+  by(transfer;
+     auto simp del:set_upt simp add:List.upt_def)+
+
+(* EIP615 instructions *)
+definition eip615_codes where
+"eip615_codes = set (List.upt 0xb0 0xba)"
+declare eip615_codes_def[simp]
+typedef eip615_inst = eip615_codes by auto
+setup_lifting type_definition_eip615_inst
+
+lift_definition EIP615_JUMPTO    :: "eip615_inst" is "0xb0" by auto
+lift_definition EIP615_JUMPIF    :: "eip615_inst" is "0xb1" by auto
+lift_definition EIP615_JUMPV     :: "eip615_inst" is "0xb2" by auto
+lift_definition EIP615_JUMPSUB   :: "eip615_inst" is "0xb3" by auto
+lift_definition EIP615_JUMPSUBV  :: "eip615_inst" is "0xb4" by auto
+lift_definition EIP615_BEGINSUB  :: "eip615_inst" is "0xb5" by auto
+lift_definition EIP615_BEGINDATA :: "eip615_inst" is "0xb6" by auto
+lift_definition EIP615_RETURNSUB :: "eip615_inst" is "0xb7" by auto
+lift_definition EIP615_PUTLOCAL  :: "eip615_inst" is "0xb8" by auto
+lift_definition EIP615_GETLOCAL  :: "eip615_inst" is "0xb9" by auto
+
+free_constructors cases_eip615_inst for
+EIP615_JUMPTO
+| EIP615_JUMPIF
+| EIP615_JUMPV
+| EIP615_JUMPSUB
+| EIP615_JUMPSUBV
+| EIP615_BEGINSUB
+| EIP615_BEGINDATA
+| EIP615_RETURNSUB
+| EIP615_PUTLOCAL
+| EIP615_GETLOCAL
+  by(transfer;
+     auto simp del:set_upt simp add:List.upt_def)+
+
+(* cross-contract communication instructions *)
+definition comms_codes where
+"comms_codes = set (List.upt 0xf0 0xf6) \<union> {0xfa}"
+declare comms_codes_def[simp]
+typedef comms_inst = comms_codes by auto
+setup_lifting type_definition_comms_inst
+
+lift_definition COMMS_CREATE       :: "comms_inst" is "0xf0" by auto
+lift_definition COMMS_CALL         :: "comms_inst" is "0xf1" by auto
+lift_definition COMMS_CALLCODE     :: "comms_inst" is "0xf2" by auto
+lift_definition COMMS_RETURN       :: "comms_inst" is "0xf3" by auto
+lift_definition COMMS_DELEGATECALL :: "comms_inst" is "0xf4" by auto
+lift_definition COMMS_CREATE2      :: "comms_inst" is "0xf5" by auto
+lift_definition COMMS_STATICCALL   :: "comms_inst" is "0xfa" by auto
+
+free_constructors cases_comms_inst for
+COMMS_CREATE
+| COMMS_CALL
+| COMMS_CALLCODE
+| COMMS_RETURN
+| COMMS_DELEGATECALL
+| COMMS_CREATE2
+| COMMS_STATICCALL
+  by(transfer;
+     auto simp del:set_upt simp add:List.upt_def)+
+
+(* special halting instructions *)
+definition special_halt_codes where
+"special_halt_codes = set (List.upt 0xfd 0x100)"
+declare special_halt_codes_def[simp]
+typedef special_halt_inst = special_halt_codes by auto
+setup_lifting type_definition_special_halt_inst
+
+lift_definition SPECIAL_HALT_REVERT       :: "special_halt_inst" is "0xfd" by auto
+lift_definition SPECIAL_HALT_INVALID      :: "special_halt_inst" is "0xfe" by auto
+lift_definition SPECIAL_HALT_SELFDESTRUCT :: "special_halt_inst" is "0xff" by auto
+
+free_constructors cases_special_halt_inst for
+SPECIAL_HALT_REVERT
+| SPECIAL_HALT_INVALID
+| SPECIAL_HALT_SELFDESTRUCT
+  by(transfer;
+     auto simp del:set_upt simp add:List.upt_def)+
+
+(* putting it all together *)
+
+(* we are leaving out EIP615 *)
+definition good_inst_codes :: "nat set" where
+"good_inst_codes = 
+  stop_codes \<union>
+  arith_codes \<union>
+  compare_codes \<union>
+  bits_codes \<union>
+  keccak256_codes \<union>
+  tx_data_codes \<union>
+  chain_data_codes \<union>
+  state_control_codes \<union>
+  push_few_codes \<union>
+  push_many_codes \<union>
+  dup_codes \<union>
+  swap_codes \<union>
+  log_codes \<union>
+  comms_codes \<union>
+  special_halt_codes"
+
+definition bad_inst_codes :: "nat set" where
+"bad_inst_codes = 
+  UNIV - good_inst_codes"
+  
 
 (*
 typedef stop_others = "UNIV - stop_codes" unfolding stop_codes_def by auto
 setup_lifting type_definition_stop_others
 *)
+(*
 lift_definition 
 
 
@@ -391,5 +963,7 @@ value "(\<lambda> i :: nat . (case i of (1 :: nat) \<Rightarrow> True))"
 
 
 value "3 :: 8 word"
+*)
+*)
 
 end
